re-structured proof scripts in Ackermann/codeSubTerm

theories/ordinals/Ackermann/codeSubTerm.v
@@ -6,6 +6,8 @@ Require Import code.
 Require Import extEqualNat.
 Require Vector.
 Require Import Compat815.
+Import LispAbbreviations. 
+
 
 Section Code_Substitute_Term.
 
@@ -23,421 +25,345 @@ Let apply := apply L.
 Definition codeSubTermTerms : nat -> nat -> nat -> nat :=
   evalStrongRec 2
     (fun t recs v s : nat =>
-     cPair
-       (switchPR (cPairPi1 t)
-          (cPair (cPairPi1 t) (cPairPi2 (codeNth (t - S (cPairPi2 t)) recs)))
-          (switchPR (charFunction 2 Nat.eqb (cPairPi2 t) v) s t))
-       (switchPR t
-          (S
-             (cPair (cPairPi1 (codeNth (t - S (cPairPi1 (pred t))) recs))
-                (cPairPi2 (codeNth (t - S (cPairPi2 (pred t))) recs)))) 0)).
+       cPair
+         (switchPR (car t)
+            (cPair (car t) (cdr (codeNth (t - S (cdr t)) recs)))
+            (switchPR (charFunction 2 Nat.eqb (cdr t) v) s t))
+         (switchPR t
+            (S
+               (cPair (car (codeNth (t - S (car (pred t))) recs))
+                  (cdr (codeNth (t - S (cdr (pred t))) recs)))) 0)).
 
 Definition codeSubTerm (t s v : nat) : nat :=
-  cPairPi1 (codeSubTermTerms t s v).
+  car (codeSubTermTerms t s v).
 
 Definition codeSubTerms (t s v : nat) : nat :=
-  cPairPi2 (codeSubTermTerms t s v).
+  cdr (codeSubTermTerms t s v).
 
 Lemma codeSubTermCorrect :
- forall (t : Term) (v : nat) (s : Term),
- codeSubTerm (codeTerm L codeF t) v (codeTerm L codeF s) =
- codeTerm L codeF (substituteTerm L t v s).
+  forall (t : Term) (v : nat) (s : Term),
+    codeSubTerm (codeTerm L codeF t) v (codeTerm L codeF s) =
+      codeTerm L codeF (substituteTerm L t v s).
 Proof.
-set
- (g :=
-  fun t0 recs v0 s0 : nat =>
-  cPair
-    (switchPR (cPairPi1 t0)
-       (cPair (cPairPi1 t0) (cPairPi2 (codeNth (t0 - S (cPairPi2 t0)) recs)))
-       (switchPR (charFunction 2 Nat.eqb (cPairPi2 t0) v0) s0 t0))
-    (switchPR t0
-       (S
-          (cPair (cPairPi1 (codeNth (t0 - S (cPairPi1 (pred t0))) recs))
-             (cPairPi2 (codeNth (t0 - S (cPairPi2 (pred t0))) recs)))) 0))
- in *.
-intros.
-elim t using
- Term_Terms_ind
-  with
+  set
+    (g :=
+       fun t0 recs v0 s0 : nat =>
+         cPair
+           (switchPR (car t0)
+              (cPair (car t0) (cdr (codeNth (t0 - S (cdr t0)) recs)))
+              (switchPR (charFunction 2 Nat.eqb (cdr t0) v0) s0 t0))
+           (switchPR t0
+              (S
+                 (cPair (car (codeNth (t0 - S (car (pred t0))) recs))
+                    (cdr (codeNth (t0 - S (cdr (pred t0))) recs)))) 0)).
+  
+  intros t v s; elim t using  Term_Terms_ind
+    with
     (P0 := fun (n : nat) (ts : fol.Terms L n) =>
-           codeSubTerms (codeTerms L codeF n ts) v (codeTerm L codeF s) =
-           codeTerms L codeF n (substituteTerms L n ts v s)); 
- intros.
-simpl in |- *.
-replace (codeTerm L codeF (fol.var L n)) with (cPair 0 n).
-unfold codeSubTerm in |- *.
-unfold codeSubTermTerms in |- *.
-unfold evalStrongRec in |- *.
-simpl in |- *.
-repeat rewrite cPairProjections1 || rewrite cPairProjections2.
-simpl in |- *.
-induction (eq_nat_dec v n).
-rewrite a.
-rewrite  Nat.eqb_refl.
-simpl in |- *.
-reflexivity.
-rewrite nat_eqb_false.
-simpl in |- *.
-reflexivity.
-auto.
-reflexivity.
-simpl in |- *.
-transitivity
- (cPair (S (codeF f))
-    (codeTerms L codeF (arity L (inr (Relations L) f))
-       (substituteTerms L (arity L (inr (Relations L) f)) t0 v s))).
-rewrite <- H.
-replace (codeTerm L codeF (fol.apply L f t0)) with
- (cPair (S (codeF f)) (codeTerms L codeF (arity L (inr (Relations L) f)) t0)).
-generalize (codeF f) (codeTerms L codeF (arity L (inr (Relations L) f)) t0).
-clear H t0 f.
-intros.
-unfold codeSubTerm in |- *.
-unfold codeSubTermTerms in |- *.
-fold g in |- *.
-unfold evalStrongRec in |- *.
-unfold evalComposeFunc in |- *.
-unfold evalOneParamList in |- *.
-unfold evalList in |- *.
-rewrite computeEvalStrongRecHelp.
-unfold compose2 in |- *.
-unfold evalComposeFunc, evalOneParamList, evalList in |- *.
-unfold pred in |- *.
-repeat rewrite cPairProjections1 || rewrite cPairProjections2.
-unfold g at 1 in |- *.
-repeat rewrite cPairProjections1 || rewrite cPairProjections2.
-assert
- (extEqual _
-    (evalComposeFunc 2 1
-       (Vector.cons _ (evalStrongRecHelp 2 g (cPair (S n) n0)) 0 (Vector.nil _))
-       (fun b : nat => codeNth (cPair (S n) n0 - S n0) b))
-    (evalStrongRec 2 g n0)).
-apply (evalStrongRecHelp2 2).
-apply cPairLt2.
-simpl in H.
-rewrite H.
-clear H.
-simpl in |- *.
-reflexivity.
-reflexivity.
-reflexivity.
-simpl in |- *.
-unfold codeTerms in |- *.
-unfold codeSubTerms in |- *.
-unfold codeSubTermTerms in |- *.
-unfold evalStrongRec in |- *.
-simpl in |- *.
-repeat rewrite cPairProjections1 || rewrite cPairProjections2.
-reflexivity.
-simpl in |- *.
-transitivity
- (S
-    (cPair (codeTerm L codeF (substituteTerm L t0 v s))
-       (codeTerms L codeF n (substituteTerms L n t1 v s)))).
-rewrite <- H.
-rewrite <- H0.
-replace (codeTerms L codeF (S n) (Tcons L n t0 t1)) with
- (S (cPair (codeTerm L codeF t0) (codeTerms L codeF n t1))).
-generalize (codeTerm L codeF t0) (codeTerms L codeF n t1).
-clear H0 t1 H t0 n.
-intros.
-unfold codeSubTerms at 1 in |- *.
-unfold codeSubTermTerms in |- *.
-fold g in |- *.
-unfold evalStrongRec in |- *.
-unfold evalComposeFunc, evalOneParamList, evalList in |- *.
-rewrite computeEvalStrongRecHelp.
-unfold compose2 in |- *.
-unfold evalComposeFunc, evalOneParamList, evalList in |- *.
-unfold pred in |- *.
-repeat rewrite cPairProjections1 || rewrite cPairProjections2.
-unfold g at 1 in |- *.
-repeat rewrite cPairProjections1 || rewrite cPairProjections2.
-unfold pred in |- *.
-repeat rewrite cPairProjections1 || rewrite cPairProjections2.
-assert
- (extEqual _
-    (evalComposeFunc 2 1
-       (Vector.cons _ (evalStrongRecHelp 2 g (S (cPair n n0))) 0 (Vector.nil _))
-       (fun b : nat => codeNth (S (cPair n n0) - S n) b))
-    (evalStrongRec 2 g n)).
-apply (evalStrongRecHelp2 2).
-apply Compat815.le_lt_n_Sm.
-apply cPairLe1.
-simpl in H.
-rewrite H.
-clear H.
-assert
- (extEqual _
-    (evalComposeFunc 2 1
-       (Vector.cons _ (evalStrongRecHelp 2 g (S (cPair n n0))) 0 (Vector.nil _))
-       (fun b : nat => codeNth (S (cPair n n0) - S n0) b))
-    (evalStrongRec 2 g n0)).
-apply (evalStrongRecHelp2 2).
-apply Compat815.le_lt_n_Sm.
-apply cPairLe2.
-simpl in H.
-rewrite H.
-clear H.
-simpl in |- *.
-reflexivity.
-reflexivity.
-reflexivity.
+             codeSubTerms (codeTerms L codeF n ts) v (codeTerm L codeF s) =
+               codeTerms L codeF n (substituteTerms L n ts v s)).
+    - intro n; simpl; replace (codeTerm L codeF (fol.var L n)) with (cPair 0 n).
+      + unfold codeSubTerm, codeSubTermTerms, evalStrongRec; simpl.
+        repeat rewrite cPairProjections1 || rewrite cPairProjections2.
+        simpl; induction (eq_nat_dec v n) as [a | b].
+        * rewrite a, Nat.eqb_refl; simpl; reflexivity.
+        * rewrite nat_eqb_false; simpl. 
+          -- reflexivity.
+          -- auto.
+      + reflexivity.
+    - intros f t0 H; simpl;
+        transitivity
+          (cPair (S (codeF f))
+             (codeTerms L codeF (arity L (inr (Relations L) f))
+                (substituteTerms L (arity L (inr (Relations L) f)) t0 v s))).
+      + rewrite <- H; 
+          replace (codeTerm L codeF (fol.apply L f t0)) 
+          with
+          (cPair (S (codeF f)) 
+             (codeTerms L codeF (arity L (inr (Relations L) f)) t0)).
+        * generalize (codeF f) 
+            (codeTerms L codeF (arity L (inr (Relations L) f)) t0).
+          clear H t0 f; intros n n0; unfold codeSubTerm, codeSubTermTerms.
+          fold g; unfold evalStrongRec, evalComposeFunc, evalOneParamList.
+          unfold evalList; rewrite computeEvalStrongRecHelp.
+          -- unfold compose2, evalComposeFunc, evalOneParamList, evalList.
+             unfold pred;
+               repeat rewrite cPairProjections1 || rewrite cPairProjections2.
+             unfold g at 1;
+               repeat rewrite cPairProjections1 || rewrite cPairProjections2.
+             assert
+               (H: extEqual _
+                     (evalComposeFunc 2 1
+                        (Vector.cons _ 
+                           (evalStrongRecHelp 2 g (cPair (S n) n0)) 0
+                           (Vector.nil _))
+                        (fun b : nat => codeNth (cPair (S n) n0 - S n0) b))
+                     (evalStrongRec 2 g n0)) 
+               by (apply (evalStrongRecHelp2 2), cPairLt2).
+             simpl in H; rewrite H; clear H.
+             simpl; reflexivity.
+        * reflexivity.
+      + reflexivity.
+    - simpl; unfold codeTerms, codeSubTerms, codeSubTermTerms, evalStrongRec.
+      simpl;
+        repeat rewrite cPairProjections1 || rewrite cPairProjections2.
+      reflexivity.
+    - intros n t0 H t1 H0 ; simpl.
+      transitivity
+        (S (cPair (codeTerm L codeF (substituteTerm L t0 v s))
+              (codeTerms L codeF n (substituteTerms L n t1 v s)))).
+      + rewrite <- H, <-  H0.
+        replace (codeTerms L codeF (S n) (Tcons L n t0 t1)) 
+          with
+          (S (cPair (codeTerm L codeF t0) (codeTerms L codeF n t1))).
+        * generalize (codeTerm L codeF t0) (codeTerms L codeF n t1).
+          clear H0 t1 H t0 n; intros n n0.
+          unfold codeSubTerms at 1; unfold codeSubTermTerms; fold g.
+          unfold evalStrongRec, evalComposeFunc, evalOneParamList, evalList.
+          rewrite computeEvalStrongRecHelp.
+          unfold compose2, evalComposeFunc, evalOneParamList, evalList, pred.
+          repeat rewrite cPairProjections1 || rewrite cPairProjections2.
+          unfold g;
+            repeat rewrite cPairProjections1 || rewrite cPairProjections2.
+          unfold pred;
+            repeat rewrite cPairProjections1 || rewrite cPairProjections2.
+          assert
+            (H: extEqual _
+                  (evalComposeFunc 2 1
+                     (Vector.cons _ (evalStrongRecHelp 2 g 
+                                       (S (cPair n n0))) 0 (Vector.nil _))
+                     (fun b : nat => codeNth (S (cPair n n0) - S n) b))
+                  (evalStrongRec 2 g n)).
+          { apply (evalStrongRecHelp2 2).
+            apply Compat815.le_lt_n_Sm.
+            apply cPairLe1.
+          } 
+          simpl in H; rewrite H; clear H.
+          assert
+            (H: extEqual _
+                  (evalComposeFunc 2 1
+                     (Vector.cons _ 
+                        (evalStrongRecHelp 2 g (S (cPair n n0))) 0 
+                        (Vector.nil _))
+                     (fun b : nat => codeNth (S (cPair n n0) - S n0) b))
+                  (evalStrongRec 2 g n0)).
+          { apply (evalStrongRecHelp2 2).
+            apply Compat815.le_lt_n_Sm.
+            apply cPairLe2.
+          } 
+          simpl in H; rewrite H; clear H; simpl.
+          reflexivity.
+        * reflexivity.
+      + reflexivity.
 Qed.
 
 Lemma codeSubTermsCorrect :
- forall (n : nat) (ts : Terms n) (v : nat) (s : Term),
- codeSubTerms (codeTerms L codeF n ts) v (codeTerm L codeF s) =
- codeTerms L codeF n (substituteTerms L n ts v s).
+  forall (n : nat) (ts : Terms n) (v : nat) (s : Term),
+    codeSubTerms (codeTerms L codeF n ts) v (codeTerm L codeF s) =
+      codeTerms L codeF n (substituteTerms L n ts v s).
 Proof.
-set
- (g :=
-  fun t0 recs v0 s0 : nat =>
-  cPair
-    (switchPR (cPairPi1 t0)
-       (cPair (cPairPi1 t0) (cPairPi2 (codeNth (t0 - S (cPairPi2 t0)) recs)))
-       (switchPR (charFunction 2 Nat.eqb (cPairPi2 t0) v0) s0 t0))
-    (switchPR t0
-       (S
-          (cPair (cPairPi1 (codeNth (t0 - S (cPairPi1 (pred t0))) recs))
-             (cPairPi2 (codeNth (t0 - S (cPairPi2 (pred t0))) recs)))) 0))
- in *.
-intros.
-induction ts as [| n t ts Hrects].
-simpl in |- *.
-unfold codeTerms in |- *.
-unfold codeSubTerms in |- *.
-unfold codeSubTermTerms in |- *.
-unfold evalStrongRec in |- *.
-simpl in |- *.
-repeat rewrite cPairProjections1 || rewrite cPairProjections2.
-reflexivity.
-simpl in |- *.
-transitivity
- (S
-    (cPair (codeTerm L codeF (substituteTerm L t v s))
-       (codeTerms L codeF n (substituteTerms L n ts v s)))).
-rewrite <- Hrects.
-rewrite <- codeSubTermCorrect.
-replace (codeTerms L codeF (S n) (Tcons L n t ts)) with
- (S (cPair (codeTerm L codeF t) (codeTerms L codeF n ts))).
-generalize (codeTerm L codeF t) (codeTerms L codeF n ts).
-clear Hrects ts t n.
-intros.
-unfold codeSubTerms at 1 in |- *.
-unfold codeSubTermTerms in |- *.
-fold g in |- *.
-unfold evalStrongRec in |- *.
-unfold evalComposeFunc, evalOneParamList, evalList in |- *.
-rewrite computeEvalStrongRecHelp.
-unfold compose2 in |- *.
-unfold evalComposeFunc, evalOneParamList, evalList in |- *.
-unfold pred in |- *.
-repeat rewrite cPairProjections1 || rewrite cPairProjections2.
-unfold g at 1 in |- *.
-repeat rewrite cPairProjections1 || rewrite cPairProjections2.
-unfold pred in |- *.
-repeat rewrite cPairProjections1 || rewrite cPairProjections2.
-assert
- (extEqual _
-    (evalComposeFunc 2 1
-       (Vector.cons _ (evalStrongRecHelp 2 g (S (cPair n n0))) 0 (Vector.nil _))
-       (fun b : nat => codeNth (S (cPair n n0) - S n) b))
-    (evalStrongRec 2 g n)).
-apply (evalStrongRecHelp2 2).
-apply Compat815.le_lt_n_Sm.
-apply cPairLe1.
-simpl in H.
-rewrite H.
-clear H.
-assert
- (extEqual _
-    (evalComposeFunc 2 1
-       (Vector.cons _ (evalStrongRecHelp 2 g (S (cPair n n0))) 0 (Vector.nil _))
-       (fun b : nat => codeNth (S (cPair n n0) - S n0) b))
-    (evalStrongRec 2 g n0)).
-apply (evalStrongRecHelp2 2).
-apply Compat815.le_lt_n_Sm.
-apply cPairLe2.
-simpl in H.
-rewrite H.
-clear H.
-simpl in |- *.
-reflexivity.
-reflexivity.
-reflexivity.
+  set
+    (g :=
+       fun t0 recs v0 s0 : nat =>
+         cPair
+           (switchPR (car t0)
+              (cPair (car t0) (cdr (codeNth (t0 - S (cdr t0)) recs)))
+              (switchPR (charFunction 2 Nat.eqb (cdr t0) v0) s0 t0))
+           (switchPR t0
+              (S
+                 (cPair (car (codeNth (t0 - S (car (pred t0))) recs))
+                    (cdr (codeNth (t0 - S (cdr (pred t0))) recs)))) 0)).
+  intros n ts v s; induction ts as [| n t ts Hrects].
+  - simpl; unfold codeTerms, codeSubTerms, codeSubTermTerms, evalStrongRec.
+    simpl; repeat rewrite cPairProjections1 || rewrite cPairProjections2.
+    reflexivity.
+  - simpl; transitivity
+             (S (cPair (codeTerm L codeF (substituteTerm L t v s))
+                   (codeTerms L codeF n (substituteTerms L n ts v s)))).
+    + rewrite <- Hrects, <- codeSubTermCorrect.
+      replace (codeTerms L codeF (S n) (Tcons L n t ts)) with
+        (S (cPair (codeTerm L codeF t) (codeTerms L codeF n ts))).
+      * generalize (codeTerm L codeF t) (codeTerms L codeF n ts).
+        clear Hrects ts t n; intros n n0.
+        unfold codeSubTerms at 1; unfold codeSubTermTerms; fold g.
+        unfold evalStrongRec, evalComposeFunc, evalOneParamList, evalList.
+        rewrite computeEvalStrongRecHelp.
+        unfold compose2, evalComposeFunc, evalOneParamList, evalList.
+        unfold pred;
+          repeat rewrite cPairProjections1 || rewrite cPairProjections2.
+        unfold g at 1; 
+          repeat rewrite cPairProjections1 || rewrite cPairProjections2.
+        unfold pred;
+          repeat rewrite cPairProjections1 || rewrite cPairProjections2.
+        assert
+          (H:
+            extEqual _
+               (evalComposeFunc 2 1
+                  (Vector.cons _ (evalStrongRecHelp 2 g (S (cPair n n0))) 0 
+                     (Vector.nil _))
+                  (fun b : nat => codeNth (S (cPair n n0) - S n) b))
+               (evalStrongRec 2 g n)).
+        { apply (evalStrongRecHelp2 2).
+          apply Compat815.le_lt_n_Sm.
+          apply cPairLe1.
+        } 
+        simpl in H; rewrite H; clear H.
+        assert
+          (H: extEqual _
+                (evalComposeFunc 2 1
+                   (Vector.cons _ (evalStrongRecHelp 2 g 
+                                     (S (cPair n n0))) 0 (Vector.nil _))
+                   (fun b : nat => codeNth (S (cPair n n0) - S n0) b))
+                (evalStrongRec 2 g n0)).
+        { apply (evalStrongRecHelp2 2).
+          apply Compat815.le_lt_n_Sm.
+          apply cPairLe2.
+        } 
+        simpl in H; rewrite H; clear H.
+        simpl; reflexivity.
+      * reflexivity.
+    + reflexivity.
 Qed.
 
 Lemma codeSubTermTermsIsPR : isPR 3 codeSubTermTerms.
 Proof.
-unfold codeSubTermTerms in |- *.
-apply evalStrongRecIsPR.
-apply
- compose4_2IsPR
-  with
+  unfold codeSubTermTerms; apply evalStrongRecIsPR.
+  apply compose4_2IsPR with
     (f1 := fun t recs v s : nat =>
-           switchPR (cPairPi1 t)
-             (cPair (cPairPi1 t)
-                (cPairPi2 (codeNth (t - S (cPairPi2 t)) recs)))
-             (switchPR (charFunction 2 Nat.eqb (cPairPi2 t) v) s t))
+             switchPR (car t)
+               (cPair (car t)
+                  (cdr (codeNth (t - S (cdr t)) recs)))
+               (switchPR (charFunction 2 Nat.eqb (cdr t) v) s t))
     (f2 := fun t recs v s : nat =>
-           switchPR t
-             (S
-                (cPair (cPairPi1 (codeNth (t - S (cPairPi1 (pred t))) recs))
-                   (cPairPi2 (codeNth (t - S (cPairPi2 (pred t))) recs)))) 0).
-apply
- compose4_3IsPR
-  with
-    (f1 := fun t recs v s : nat => cPairPi1 t)
-    (f2 := fun t recs v s : nat =>
-           cPair (cPairPi1 t) (cPairPi2 (codeNth (t - S (cPairPi2 t)) recs)))
-    (f3 := fun t recs v s : nat =>
-           switchPR (charFunction 2 Nat.eqb (cPairPi2 t) v) s t).
-apply filter1000IsPR with (g := cPairPi1).
-apply cPairPi1IsPR.
-apply
- filter1100IsPR
-  with
-    (g := fun t recs : nat =>
-          cPair (cPairPi1 t) (cPairPi2 (codeNth (t - S (cPairPi2 t)) recs))).
-apply
- compose2_2IsPR
-  with
-    (f := fun t recs : nat => cPairPi1 t)
-    (g := fun t recs : nat => cPairPi2 (codeNth (t - S (cPairPi2 t)) recs)).
-apply filter10IsPR with (g := cPairPi1).
-apply cPairPi1IsPR.
-apply
- compose2_1IsPR
-  with (f := fun t recs : nat => codeNth (t - S (cPairPi2 t)) recs).
-apply
- compose2_2IsPR
-  with
-    (f := fun t recs : nat => t - S (cPairPi2 t))
-    (g := fun t recs : nat => recs).
-apply filter10IsPR with (g := fun t : nat => t - S (cPairPi2 t)).
-apply
- compose1_2IsPR
-  with (f := fun t : nat => t) (f' := fun t : nat => S (cPairPi2 t)).
-apply idIsPR.
-apply compose1_1IsPR.
-apply cPairPi2IsPR.
-apply succIsPR.
-apply minusIsPR.
-apply pi2_2IsPR.
-apply codeNthIsPR.
-apply cPairPi2IsPR.
-apply cPairIsPR.
-apply
- filter1011IsPR
-  with
-    (g := fun t v s : nat =>
-          switchPR (charFunction 2 Nat.eqb (cPairPi2 t) v) s t).
-apply
- compose3_3IsPR
-  with
-    (f1 := fun t v s : nat => charFunction 2 Nat.eqb (cPairPi2 t) v)
-    (f2 := fun t v s : nat => s)
-    (f3 := fun t v s : nat => t).
-apply
- filter110IsPR
-  with (g := fun t v : nat => charFunction 2 Nat.eqb (cPairPi2 t) v).
-apply
- compose2_2IsPR
-  with (f := fun t v : nat => cPairPi2 t) (g := fun t v : nat => v).
-apply filter10IsPR.
-apply cPairPi2IsPR.
-apply pi2_2IsPR.
-apply eqIsPR.
-apply pi3_3IsPR.
-apply pi1_3IsPR.
-apply switchIsPR.
-apply switchIsPR.
-apply
- filter1100IsPR
-  with
-    (g := fun t recs : nat =>
-          switchPR t
-            (S
-               (cPair (cPairPi1 (codeNth (t - S (cPairPi1 (pred t))) recs))
-                  (cPairPi2 (codeNth (t - S (cPairPi2 (pred t))) recs)))) 0).
-apply
- compose2_3IsPR
-  with
-    (f1 := fun t recs : nat => t)
-    (f2 := fun t recs : nat =>
-           S
-             (cPair (cPairPi1 (codeNth (t - S (cPairPi1 (pred t))) recs))
-                (cPairPi2 (codeNth (t - S (cPairPi2 (pred t))) recs))))
-    (f3 := fun t recs : nat => 0).
-apply pi1_2IsPR.
-apply
- compose2_1IsPR
-  with
-    (f := fun t recs : nat =>
-          cPair (cPairPi1 (codeNth (t - S (cPairPi1 (pred t))) recs))
-            (cPairPi2 (codeNth (t - S (cPairPi2 (pred t))) recs))).
-assert
- (forall g : nat -> nat,
-  isPR 1 g ->
-  isPR 2 (fun t recs : nat => g (codeNth (t - S (g (pred t))) recs))).
-intros.
-apply
- compose2_1IsPR
-  with (f := fun t recs : nat => codeNth (t - S (g (pred t))) recs).
-apply
- compose2_2IsPR
-  with
-    (f := fun t recs : nat => t - S (g (pred t)))
-    (g := fun t recs : nat => recs).
-apply filter10IsPR with (g := fun t : nat => t - S (g (pred t))).
-apply
- compose1_2IsPR
-  with (f := fun t : nat => t) (f' := fun t : nat => S (g (pred t))).
-apply idIsPR.
-apply compose1_1IsPR with (f := fun t : nat => g (pred t)).
-apply compose1_1IsPR.
-apply predIsPR.
-auto.
-apply succIsPR.
-apply minusIsPR.
-apply pi2_2IsPR.
-apply codeNthIsPR.
-auto.
-apply
- compose2_2IsPR
-  with
-    (f := fun t recs : nat =>
-          cPairPi1 (codeNth (t - S (cPairPi1 (pred t))) recs))
-    (g := fun t recs : nat =>
-          cPairPi2 (codeNth (t - S (cPairPi2 (pred t))) recs)).
-apply H.
-apply cPairPi1IsPR.
-apply H.
-apply cPairPi2IsPR.
-apply cPairIsPR.
-apply succIsPR.
-exists (composeFunc 2 0 (PRnil _) zeroFunc).
-simpl in |- *.
-auto.
-apply switchIsPR.
-apply cPairIsPR.
+             switchPR t
+               (S
+                  (cPair (car (codeNth (t - S (car (pred t))) recs))
+                     (cdr (codeNth (t - S (cdr (pred t))) recs)))) 0).
+  - apply compose4_3IsPR with
+      (f1 := fun t recs v s : nat => car t)
+      (f2 := fun t recs v s : nat =>
+               cPair (car t) (cdr (codeNth (t - S (cdr t)) recs)))
+      (f3 := fun t recs v s : nat =>
+               switchPR (charFunction 2 Nat.eqb (cdr t) v) s t).
+    + apply filter1000IsPR with (g := cPairPi1).
+      apply cPairPi1IsPR.
+    + apply filter1100IsPR with
+        (g := fun t recs : nat =>
+                cPair (car t) (cdr (codeNth (t - S (cdr t)) recs))).
+      apply compose2_2IsPR with
+        (f := fun t recs : nat => car t)
+        (g := fun t recs : nat => cdr (codeNth (t - S (cdr t)) recs)).
+      * apply filter10IsPR with (g := cPairPi1).
+        apply cPairPi1IsPR.
+      * apply compose2_1IsPR with 
+          (f := fun t recs : nat => codeNth (t - S (cdr t)) recs).
+        -- apply compose2_2IsPR with
+             (f := fun t recs : nat => t - S (cdr t))
+             (g := fun t recs : nat => recs).
+           ++ apply filter10IsPR with (g := fun t : nat => t - S (cdr t)).
+              apply compose1_2IsPR with
+                (f := fun t : nat => t) (f' := fun t : nat => S (cdr t)).
+              ** apply idIsPR.
+              ** apply compose1_1IsPR.
+                 apply cPairPi2IsPR.
+                 apply succIsPR.
+              ** apply minusIsPR.
+           ++ apply pi2_2IsPR.
+           ++ apply codeNthIsPR.
+        -- apply cPairPi2IsPR.
+      * apply cPairIsPR.
+    + apply filter1011IsPR with
+        (g := fun t v s : nat =>
+                switchPR (charFunction 2 Nat.eqb (cdr t) v) s t).
+      apply compose3_3IsPR with
+        (f1 := fun t v s : nat => charFunction 2 Nat.eqb (cdr t) v)
+        (f2 := fun t v s : nat => s)
+        (f3 := fun t v s : nat => t).
+      * apply filter110IsPR with 
+          (g := fun t v : nat => charFunction 2 Nat.eqb (cdr t) v).
+        apply compose2_2IsPR with 
+          (f := fun t v : nat => cdr t) (g := fun t v : nat => v).
+        -- apply filter10IsPR.
+           apply cPairPi2IsPR.
+        -- apply pi2_2IsPR.
+        -- apply eqIsPR.
+      * apply pi3_3IsPR.
+      * apply pi1_3IsPR.
+      * apply switchIsPR.
+    + apply switchIsPR.
+  - apply filter1100IsPR with
+      (g := fun t recs : nat =>
+              switchPR t
+                (S
+                   (cPair (car (codeNth (t - S (car (pred t))) recs))
+                      (cdr (codeNth (t - S (cdr (pred t))) recs)))) 0).
+    apply compose2_3IsPR with
+      (f1 := fun t recs : nat => t)
+      (f2 := fun t recs : nat =>
+               S
+                 (cPair (car (codeNth (t - S (car (pred t))) recs))
+                    (cdr (codeNth (t - S (cdr (pred t))) recs))))
+      (f3 := fun t recs : nat => 0).
+    + apply pi1_2IsPR.
+    + apply compose2_1IsPR with
+        (f := fun t recs : nat =>
+                cPair (car (codeNth (t - S (car (pred t))) recs))
+                  (cdr (codeNth (t - S (cdr (pred t))) recs))).
+      * assert
+          (H: forall g : nat -> nat,
+              isPR 1 g ->
+              isPR 2 (fun t recs : nat => 
+                        g (codeNth (t - S (g (pred t))) recs))).
+        { intros g H;
+            apply compose2_1IsPR with 
+            (f := fun t recs : nat => codeNth (t - S (g (pred t))) recs).
+          - apply compose2_2IsPR with
+              (f := fun t recs : nat => t - S (g (pred t)))
+              (g := fun t recs : nat => recs).
+            + apply filter10IsPR with 
+                (g := fun t : nat => t - S (g (pred t))).
+              apply compose1_2IsPR with 
+                (f := fun t : nat => t) (f' := fun t : nat => S (g (pred t))).
+              * apply idIsPR.
+              * apply compose1_1IsPR with (f := fun t : nat => g (pred t)).
+                -- apply compose1_1IsPR.
+                   ++ apply predIsPR.
+                   ++ auto.
+                -- apply succIsPR.
+              * apply minusIsPR.
+            + apply pi2_2IsPR.
+            + apply codeNthIsPR.
+          - auto.
+        } 
+        apply compose2_2IsPR with
+          (f := fun t recs : nat =>
+                  car (codeNth (t - S (car (pred t))) recs))
+          (g := fun t recs : nat =>
+                  cdr (codeNth (t - S (cdr (pred t))) recs)).
+        -- apply H.
+           apply cPairPi1IsPR.
+        -- apply H.
+           apply cPairPi2IsPR.
+        -- apply cPairIsPR.
+      * apply succIsPR.
+    + exists (composeFunc 2 0 (PRnil _) zeroFunc).
+      simpl; auto.
+    + apply switchIsPR.
+  - apply cPairIsPR.
 Qed.
 
 Lemma codeSubTermIsPR : isPR 3 codeSubTerm.
 Proof.
-unfold codeSubTerm in |- *.
-apply compose3_1IsPR.
-apply codeSubTermTermsIsPR.
-apply cPairPi1IsPR.
+  unfold codeSubTerm; apply compose3_1IsPR.
+  - apply codeSubTermTermsIsPR.
+  - apply cPairPi1IsPR.
 Qed.
 
 Lemma codeSubTermsIsPR : isPR 3 codeSubTerms.
 Proof.
-unfold codeSubTerms in |- *.
-apply compose3_1IsPR.
-apply codeSubTermTermsIsPR.
-apply cPairPi2IsPR.
+  unfold codeSubTerms; apply compose3_1IsPR.
+  - apply codeSubTermTermsIsPR.
+  - apply cPairPi2IsPR.
 Qed.
 
 End Code_Substitute_Term.
